feat: prove that regular languages are closed under concatenation (#239)
In this patch we prove that regular languages are closed under
concatenation, by leveraging the results already proved about the
infinite executions of the automata concatenation construction in
`NA/Concat.lean`. In order to do so, we introduce the notion of a "total
LTS", which means that the LTS has a next state for any given starting
state and label, and a "LTS.totalize" construction that converts any LTS
into a total LTS by adding a sink state and transitions from all states
to the sink state. Then the notion of "total" and the "totalize"
construction are generalized to NA. By "totalizing" NA's, we can extend
any finite execution of a NA into an infinite execution and thus re-use
the results already proved for infinite executions.

The same technique can be applied to `NA/Loop.lean` to prove that
regular languages are closed under the Kleene star; see PR
https://github.com/leanprover/cslib/pull/241.

Cslib/Computability/Automata/NA/Concat.lean
@@ -4,7 +4,7 @@ Released under Apache 2.0 license as described in the file LICENSE.
 Authors: Ching-Tsun Chou
 -/
 
-import Cslib.Computability.Automata.NA.Basic
+import Cslib.Computability.Automata.NA.Total
 import Cslib.Foundations.Data.OmegaSequence.Temporal
 
 /-! # Concatenation of nondeterministic automata. -/
@@ -74,17 +74,18 @@ lemma concat_run_right {xs : ωSequence Symbol} {ss : ωSequence (State1 ⊕ Sta
 
 /-- A run of `concat na1 na2` containing at least one `na2` state is the concatenation of
 an accepting finite run of `na1` followed by a run of `na2`. -/
-theorem concat_run_proj {xs : ωSequence Symbol} {ss : ωSequence (State1 ⊕ State2)}
-    (hc : (concat na1 na2).Run xs ss) (hr : ∃ k, (ss k).isRight) :
-    ∃ n, xs.take n ∈ language na1 ∧ ∃ ss2, na2.Run (xs.drop n) ss2 ∧ ss.drop n = ss2.map inr := by
-  let n := Nat.find hr
-  have hl (k) (h_k : k < n) := not_isRight.mp <| Nat.find_min hr h_k
-  refine ⟨n, ?_, ?_⟩
+theorem concat_run_proj {xs : ωSequence Symbol} {ss : ωSequence (State1 ⊕ State2)} {k : ℕ}
+    (hc : (concat na1 na2).Run xs ss) (hr : (ss k).isRight) :
+    ∃ n, n ≤ k ∧ xs.take n ∈ language na1 ∧
+    ∃ ss2, na2.Run (xs.drop n) ss2 ∧ ss.drop n = ss2.map inr := by
+  have hr' : ∃ k, (ss k).isRight := by grind
+  let n := Nat.find hr'
+  have hl (k) (h_k : k < n) := not_isRight.mp <| Nat.find_min hr' h_k
+  refine ⟨n, by grind, ?_, ?_⟩
   · by_cases h_n : n = 0
     · grind [concat_start_right]
     · grind [concat_run_left_right]
-  · have hr : (ss n).isRight := Nat.find_spec hr
-    grind [concat_run_right hc n hl hr]
+  · exact concat_run_right hc n hl (Nat.find_spec hr')
 
 /-- Given an accepting finite run of `na1` and a run of `na2`, there exists a run of
 `concat na1 na2` that is the concatenation of the two runs. -/
@@ -117,8 +118,8 @@ theorem concat_language_eq {acc2 : Set State2} :
   ext xs
   constructor
   · rintro ⟨ss, h_run, h_acc⟩
-    have h_ex2 : ∃ k, (ss k).isRight := by grind [Frequently.exists h_acc]
-    obtain ⟨n, h_acc1, ss2, h_run2, h_map2⟩ := concat_run_proj h_run h_ex2
+    obtain ⟨k, h_k⟩ : ∃ k, (ss k).isRight := by grind [Frequently.exists h_acc]
+    obtain ⟨n, _, h_acc1, ss2, h_run2, h_map2⟩ := concat_run_proj h_run h_k
     use xs.take n, h_acc1, xs.drop n, ?_, by simp
     use ss2, h_run2
     grind [(drop_frequently_iff_frequently n).mpr h_acc]
@@ -129,5 +130,49 @@ theorem concat_language_eq {acc2 : Set State2} :
     grind
 
 end Buchi
+
+namespace FinAcc
+
+/-- `finConcat na1 na2` is the concatenation of the "totalized" versions of `na1` and `na2`. -/
+def finConcat (na1 : FinAcc State1 Symbol) (na2 : FinAcc State2 Symbol)
+  : NA ((State1 ⊕ Unit) ⊕ (State2 ⊕ Unit)) Symbol :=
+  concat ⟨na1.totalize, inl '' na1.accept⟩ na2.totalize
+
+variable {na1 : FinAcc State1 Symbol} {na2 : FinAcc State2 Symbol}
+
+/-- `finConcat na1 na2` is total. -/
+instance : (finConcat na1 na2).Total where
+  total s x := match s with
+    | inl _ => ⟨inl (inr ()), by grind [finConcat, concat, NA.totalize, LTS.totalize]⟩
+    | inr _ => ⟨inr (inr ()), by grind [finConcat, concat, NA.totalize, LTS.totalize]⟩
+
+/-- `finConcat na1 na2` accepts the concatenation of the languages of `na1` and `na2`. -/
+theorem finConcat_language_eq [Inhabited Symbol] :
+    language (FinAcc.mk (finConcat na1 na2) (inr '' (inl '' na2.accept))) =
+    language na1 * language na2 := by
+  ext xl
+  constructor
+  · rintro ⟨s, _, t, h_acc, h_mtr⟩
+    obtain ⟨xs, ss, h_ωtr, rfl, rfl⟩ := LTS.Total.mTr_ωTr h_mtr
+    have hc : (finConcat na1 na2).Run (xl ++ω xs) ss := by grind [Run]
+    have hr : (ss xl.length).isRight := by grind
+    obtain ⟨n, _⟩ := concat_run_proj hc hr
+    refine ⟨xl.take n, ?_, xl.drop n, ?_, ?_⟩
+    · grind [totalize_language_eq, take_append_of_le_length]
+    · have : ss xl.length = (ss.drop n) (xl.length - n) := by grind
+      grind [drop_append_of_le_length, take_append_of_le_length, totalize_run_mtr]
+    · exact xl.take_append_drop n
+  · rintro ⟨xl1, h_xl1, xl2, h_xl2, rfl⟩
+    rw [← totalize_language_eq] at h_xl1
+    obtain ⟨_, h_s2, _, _, h_mtr2⟩ := h_xl2
+    obtain ⟨_, _, h_run2, _, _⟩ := totalize_mtr_run h_s2 h_mtr2
+    obtain ⟨ss, ⟨_, h_ωtr⟩, _⟩ := concat_run_exists h_xl1 h_run2
+    grind [
+      finConcat, List.length_append, take_append_of_le_length,
+      extract_eq_drop_take, =_ append_append_ωSequence, get_drop xl2.length xl1.length ss,
+      LTS.ωTr_mTr h_ωtr (zero_le (xl1.length + xl2.length))
+    ]
+
+end FinAcc
 
 end Cslib.Automata.NA
