Cslib.lean
@@ -17,6 +17,7 @@ import Cslib.Computability.Automata.NA.Loop
 import Cslib.Computability.Automata.NA.Prod
 import Cslib.Computability.Automata.NA.Sum
 import Cslib.Computability.Automata.NA.ToDA
+import Cslib.Computability.Automata.NA.Total
 import Cslib.Computability.Languages.ExampleEventuallyZero
 import Cslib.Computability.Languages.Language
 import Cslib.Computability.Languages.OmegaLanguage
